src/Key_lt_order.thy
@@ -8,6 +8,16 @@ definition total_order_key_lte :: " bool" where
    (key_le a b \<and> key_le b c \<longrightarrow> key_le a c) \<and>
    (key_le a b \<or> key_le b a))"
 
+lemma order_key_le: "\<forall> a b c. total_order_key_lte \<longrightarrow> key_le a b \<and> key_lt b c \<longrightarrow> key_lt a c"
+apply rule+
+apply (unfold total_order_key_lte_def)
+apply (drule_tac x=a in spec)
+apply (drule_tac x=b in spec)
+apply (drule_tac x=c in spec)
+apply (simp add:key_le_def)
+apply auto
+done
+
 lemma order_key_lt: "\<forall> a b c. total_order_key_lte \<longrightarrow> key_lt a b \<and> key_lt b c \<longrightarrow> key_lt a c"
 apply (simp add:total_order_key_lte_def key_le_def,auto)
 done
